examples/lean-to-typescript/roundtrip/Sign/generated/TSLean/Examples/Roundtrip/Sign.ts
@@ -4,8 +4,8 @@
  * Lean module: TSLean.Examples.Roundtrip.Sign
  * Generated module: TSLean/Examples/Roundtrip/Sign.ts
  * Package entry module: TSLean.Examples.Roundtrip.Sign
- * Semantic identity: sha256:5e871690513fe2a18574758520a12fe7819502b707bc7708ac1a1b21c4357b66
- * Input closure: sha256:0873fd671e4c12696bb0f00397b6a039a1484c66a8110632b93b9d7c675f4e4d
+ * Semantic identity: sha256:84016bf22c543fb47f18d66269dbc357a2c73cfe88b3b819709ea9aa57c22881
+ * Input closure: sha256:07f1b657eba464a17c466ea2186fefef2cf7371cd6e905aae8e4fea4d290e1ef
  * Semantic IR: sha256:43a391ec3313f5d3cd7e78816c4bcdef5db41b290e45bc665c1b39ccbeab78e9
  * Generated module body: sha256:1aa96220b1a46b2d35fd54a2e12b5db0b2297895fb08b3c719a6bd1623be1728
  * Generated package body: sha256:b13b2ce1b97438fa3fcfb75afb820c5312ff8f920a64eb7b0f2ef2172d9530cf
